Make bvp_live delete dead code; run bvp_simp after bvp_live
The bvp_live transformation can only delete pure expressions.
Unfortunately, Cons and arithmetic (Add, Sub, etc.) cannot be
deleted because they touch the space component of the state,
i.e. they are stateful.

In the future we might consider adding a switch to the BVP
semantics which allows turning off the space component.
The bvp_space optimisation (which is run after bvp_live)
could turn on the space state component.

compiler/backend/bvp_liveScript.sml
@@ -4,7 +4,24 @@ val _ = new_theory "bvp_live";
 
 (* This script defines an optimisation that minimises the live var
    annotations that are attached to MakeSpace, Assign and Call in BVP
-   programs. *)
+   programs. It also deletes dead code. *)
+
+val is_pure_def = Define `
+  (is_pure SetGlobalsPtr = F) /\
+  (is_pure Ref = F) /\
+  (is_pure RefByte = F) /\
+  (is_pure RefArray = F) /\
+  (is_pure Update = F) /\
+  (is_pure UpdateByte = F) /\
+  (is_pure (Cons _) = F) /\
+  (is_pure (FFI _) = F) /\
+  (is_pure (FromList _) = F) /\
+  (is_pure Add = F) /\
+  (is_pure Sub = F) /\
+  (is_pure Mult = F) /\
+  (is_pure Div = F) /\
+  (is_pure Mod = F) /\
+  (is_pure _ = T)`
 
 val compile_def = Define `
   (compile Skip live = (Skip,live)) /\
@@ -20,8 +37,9 @@ val compile_def = Define `
   (compile (MakeSpace k names) live =
      let l1 = inter names live in (MakeSpace k l1,l1)) /\
   (compile (Assign v op vs NONE) live =
-     let l1 = list_insert vs (delete v live) in
-       (Assign v op vs NONE,l1)) /\
+     if IS_NONE (lookup v live) /\ is_pure op then (Skip,live) else
+       let l1 = list_insert vs (delete v live) in
+         (Assign v op vs NONE,l1)) /\
   (compile (Assign v op vs (SOME names)) live =
      let l1 = inter names (list_insert vs (delete v live)) in
        (Assign v op vs (SOME l1),l1)) /\
